export/examples/lib.thy
@@ -1,10 +1,10 @@
-theory Export
-imports Rustabelle
+theory lib
+imports "../../Rustabelle"
 begin
 
 
 
-definition fac_16 where "fac_16 res = (λ(res, iter). let t_8 = core_iter_ops_Range_A__Iterator_next in
+definition examples_fac_16 where "examples_fac_16 res = (λ(res, iter). let t_8 = core_iter_ops_Range_A__Iterator_next in
 let t_10 = iter in
 let t_9 = t_10 in
 let (t_7, t_9) = (t_8 t_9) in
@@ -15,8 +15,8 @@ let t_10 = t_9 in
 let iter = t_10 in
 ((res, iter), True))"
 
-definition fac :: "u32 => u32" where
-"fac n = (let n = n in
+definition examples_fac :: "u32 => u32" where
+"examples_fac n = (let n = n in
 let res = 1 in
 let t_3 = core_iter_I_IntoIterator_into_iter in
 let t_6 = n in
@@ -24,7 +24,7 @@ let t_5 = (t_6 + 1) in
 let t_4 = (core_ops_Range 2 t_5) in
 let (t_2) = (t_3 t_4) in
 let iter = t_2 in
-let (res, iter) = loop (fac_16 res) (res, iter) in
+let (res, iter) = loop (examples_fac_16 res) (res, iter) in
 let t_14 = res in
 let ret = t_14 in
 ret)"
