prove/examples.thy
@@ -1,14 +1,14 @@
-theory Prove
-imports Export Binomial
+theory examples
+imports "../export/examples/lib" Binomial
 begin
 
-lemma fac: "fac (n::u32) = fact n"
+lemma fac: "examples_fac (n::u32) = fact n"
 proof-
   show ?thesis
-  unfolding fac_def
+  unfolding examples_fac_def
   apply auto
   apply (rule loop_rule[where P="\<lambda>s. case s of (res,core_ops_Range (Suc l) r) \<Rightarrow> res = fact l \<and> (n = 0 \<and> l = 1 \<or> l < r) \<and> r = n+1 | _ \<Rightarrow> False"])
-  unfolding fac_16_def
+  unfolding examples_fac_16_def
   apply auto[1]
   apply (auto simp add: le_less_Suc_eq split:prod.splits core_ops_Range.splits split_if_asm option.splits nat.splits)[2]
   apply (rule wf_measure[of "\<lambda>s. case s of (_,core_ops_Range l r) \<Rightarrow> r-l"])
